[femtokernel] Removed redundant instruction; updated pc's everywhere

case_study/RiscvPmp/FemtoKernel.v
@@ -131,7 +131,7 @@ Import BlockVerificationDerived2.
     Definition femto_pmpcfg_ent1_bits : Val (ty.bvec byte) := pure_pmpcfg_ent_to_bits femto_pmpcfg_ent1.
     Definition femto_pmp0cfg_bits : Val (ty.bvec 20) := bv.zext (bv.app femto_pmpcfg_ent0_bits femto_pmpcfg_ent1_bits).
                                                                
-    Definition femto_pmpentries : list PmpEntryCfg := [(femto_pmpcfg_ent0, bv.of_N 88); (femto_pmpcfg_ent1, bv.of_N femto_address_max)]%list.
+    Definition femto_pmpentries : list PmpEntryCfg := [(femto_pmpcfg_ent0, bv.of_N 80); (femto_pmpcfg_ent1, bv.of_N femto_address_max)]%list.
 
     Definition femto_mstatus := pure_mstatus_to_bits (MkMstatus User).
 
@@ -139,13 +139,11 @@ Import BlockVerificationDerived2.
     Example femtokernel_init : list AST :=
       [
         UTYPE bv.zero ra RISCV_AUIPC
-      ; ITYPE (bv.of_N 88) ra ra RISCV_ADDI
+      ; ITYPE (bv.of_N 80) ra ra RISCV_ADDI
       ; CSR MPMPADDR0 ra zero CSRRW
       ; UTYPE (bv.of_N femto_address_max) ra RISCV_LUI
       ; CSR MPMPADDR1 ra zero CSRRW
       ; UTYPE femto_pmp0cfg_bits ra RISCV_LUI
-      ; CSR MPMP0CFG ra zero CSRRW
-      ; UTYPE femto_pmp0cfg_bits ra RISCV_LUI (* TODO: remove this line and the next (duplicate to have to bother changing pcs for now *)
       ; CSR MPMP0CFG ra zero CSRRW
       ; UTYPE bv.zero ra RISCV_AUIPC
       ; ITYPE (bv.of_N 36) ra ra RISCV_ADDI
@@ -167,7 +165,7 @@ Import BlockVerificationDerived2.
     Definition addPc (l : list AST) : list (nat * AST) :=
       map (fun '(i , a) => (i * 4 , a)%nat)
           (combine (seq 0 (List.length l)) l).
-    Compute addPc (femtokernel_init ++ femtokernel_handler).
+    (* Compute addPc (femtokernel_init ++ femtokernel_handler). *)
 
     Import asn.notations.
     (* Local Notation "a '↦[' n ']' xs" := (asn.chunk (chunk_user ptstomem [a; n; xs])) (at level 79). *)
@@ -198,13 +196,13 @@ Import BlockVerificationDerived2.
       (∃ "v", x7 ↦ term_var "v")) ∗
       (asn_pmp_entries (term_list [(term_val ty_pmpcfg_ent default_pmpcfg_ent ,ₜ term_val ty_xlenbits bv.zero);
                                       (term_val ty_pmpcfg_ent default_pmpcfg_ent ,ₜ term_val ty_xlenbits bv.zero)])) ∗
-      (term_var "a" + (term_val ty_xlenbits (bv.of_N 84)) ↦ᵣ term_val ty_xlenbits (bv.of_N 42))%exp.
+      (term_var "a" + (term_val ty_xlenbits (bv.of_N 76)) ↦ᵣ term_val ty_xlenbits (bv.of_N 42))%exp.
 
     Example femtokernel_init_post : Assertion  {| wctx := [] ▻ ("a"::ty_xlenbits) ▻ ("an"::ty_xlenbits) ; wco := []%ctx |} :=
       (
-        asn.formula (formula_relop bop.eq (term_var "an") (term_var "a" + term_val ty_xlenbits (bv.of_N 88))) ∗
+        asn.formula (formula_relop bop.eq (term_var "an") (term_var "a" + term_val ty_xlenbits (bv.of_N 80))) ∗
           (∃ "v", mstatus ↦ term_var "v") ∗
-          (mtvec ↦ (term_var "a" + term_val ty_xlenbits (bv.of_N 72))) ∗
+          (mtvec ↦ (term_var "a" + term_val ty_xlenbits (bv.of_N 64))) ∗
           (∃ "v", mcause ↦ term_var "v") ∗
           (∃ "v", mepc ↦ term_var "v") ∗
           cur_privilege ↦ term_val ty_privilege User ∗
@@ -215,9 +213,9 @@ Import BlockVerificationDerived2.
           (∃ "v", x5 ↦ term_var "v") ∗
           (∃ "v", x6 ↦ term_var "v") ∗
           (∃ "v", x7 ↦ term_var "v")) ∗
-          (asn_pmp_entries (term_list [(term_val ty_pmpcfg_ent femto_pmpcfg_ent0 ,ₜ term_var "a" + term_val ty_xlenbits (bv.of_N 88));
+          (asn_pmp_entries (term_list [(term_val ty_pmpcfg_ent femto_pmpcfg_ent0 ,ₜ term_var "a" + term_val ty_xlenbits (bv.of_N 80));
                                        (term_val ty_pmpcfg_ent femto_pmpcfg_ent1 ,ₜ term_val ty_xlenbits (bv.of_N femto_address_max))])) ∗
-          (term_var "a" + (term_val ty_xlenbits (bv.of_N 84)) ↦ᵣ term_val ty_xlenbits (bv.of_N 42))
+          (term_var "a" + (term_val ty_xlenbits (bv.of_N 76)) ↦ᵣ term_val ty_xlenbits (bv.of_N 42))
       )%exp.
 
     (* (* note that this computation takes longer than directly proving sat__femtoinit below *) *)
@@ -246,9 +244,11 @@ Import BlockVerificationDerived2.
     Let W__femtohandler : World := MkWorld Σ__femtohandler []%ctx.
 
     Example femtokernel_handler_pre : Assertion {| wctx := ["a" :: ty_xlenbits]; wco := []%ctx |} :=
-        (term_var "a" = term_val ty_word (bv.of_N 72)) ∗
+      let pmpcfg := [(term_val ty_pmpcfg_ent femto_pmpcfg_ent0 ,ₜ term_var "a" + term_val ty_xlenbits (bv.of_N 16));
+                     (term_val ty_pmpcfg_ent femto_pmpcfg_ent1 ,ₜ term_val ty_xlenbits (bv.of_N femto_address_max))]%list in
+      (term_var "a" = term_val ty_word (bv.of_N 64)) ∗
       (mstatus ↦ term_val (ty.record rmstatus) {| MPP := User |}) ∗
-      (mtvec ↦ term_val ty_word (bv.of_N 72)) ∗
+      (mtvec ↦ term_val ty_word (bv.of_N 64)) ∗
       (∃ "v", mcause ↦ term_var "v") ∗
       (∃ "epc", mepc ↦ term_var "epc") ∗
       cur_privilege ↦ term_val ty_privilege Machine ∗
@@ -259,16 +259,16 @@ Import BlockVerificationDerived2.
       (∃ "v", x5 ↦ term_var "v") ∗
       (∃ "v", x6 ↦ term_var "v") ∗
       (∃ "v", x7 ↦ term_var "v")) ∗
-      (asn_pmp_entries (term_list [(term_val ty_pmpcfg_ent femto_pmpcfg_ent0 ,ₜ term_var "a" + term_val ty_xlenbits (bv.of_N 16));
-                                   (term_val ty_pmpcfg_ent femto_pmpcfg_ent1 ,ₜ term_val ty_xlenbits (bv.of_N femto_address_max))])) ∗
-      (asn_pmp_addr_access (term_list [(term_val ty_pmpcfg_ent femto_pmpcfg_ent0 ,ₜ term_var "a" + term_val ty_xlenbits (bv.of_N 16));
-                                   (term_val ty_pmpcfg_ent femto_pmpcfg_ent1 ,ₜ term_val ty_xlenbits (bv.of_N femto_address_max))]) (term_val ty_privilege User)) ∗
+      (asn_pmp_entries (term_list pmpcfg)) ∗
+      (asn_pmp_addr_access (term_list pmpcfg) (term_val ty_privilege User)) ∗
       (term_var "a" + (term_val ty_xlenbits (bv.of_N 12)) ↦ᵣ term_val ty_xlenbits (bv.of_N 42))%exp.
 
     Example femtokernel_handler_post : Assertion {| wctx := ["a" :: ty_xlenbits; "an"::ty_xlenbits]; wco := []%ctx |} :=
+      let pmpcfg := [(term_val ty_pmpcfg_ent femto_pmpcfg_ent0 ,ₜ term_var "a" + term_val ty_xlenbits (bv.of_N 16));
+                     (term_val ty_pmpcfg_ent femto_pmpcfg_ent1 ,ₜ term_val ty_xlenbits (bv.of_N femto_address_max))]%list in
       (
           (mstatus ↦ term_val (ty.record rmstatus) {| MPP := User |}) ∗
-          (mtvec ↦ term_val ty_word (bv.of_N 72)) ∗
+          (mtvec ↦ term_val ty_word (bv.of_N 64)) ∗
           (∃ "v", mcause ↦ term_var "v") ∗
           (∃ "epc", (mepc ↦ term_var "epc" ∗
                      asn.formula
@@ -282,12 +282,9 @@ Import BlockVerificationDerived2.
           (∃ "v", x5 ↦ term_var "v") ∗
           (∃ "v", x6 ↦ term_var "v") ∗
           (∃ "v", x7 ↦ term_var "v")) ∗
-          (asn_pmp_entries (term_list [(term_val ty_pmpcfg_ent femto_pmpcfg_ent0 ,ₜ term_var "a" + term_val ty_xlenbits (bv.of_N 16));
-                                       (term_val ty_pmpcfg_ent femto_pmpcfg_ent1 ,ₜ term_val ty_xlenbits (bv.of_N femto_address_max))])) ∗
-          (asn_pmp_addr_access (term_list [(term_val ty_pmpcfg_ent femto_pmpcfg_ent0 ,ₜ term_var "a" + term_val ty_xlenbits (bv.of_N 16));
-                                       (term_val ty_pmpcfg_ent femto_pmpcfg_ent1 ,ₜ term_val ty_xlenbits (bv.of_N femto_address_max))]) (term_val ty_privilege User)) ∗
-          (term_var "a" + (term_val ty_xlenbits (bv.of_N 12)) ↦ᵣ term_val ty_xlenbits (bv.of_N 42)) ∗
-        ⊤
+          (asn_pmp_entries (term_list pmpcfg)) ∗
+          (asn_pmp_addr_access (term_list pmpcfg) (term_val ty_privilege User)) ∗
+          (term_var "a" + (term_val ty_xlenbits (bv.of_N 12)) ↦ᵣ term_val ty_xlenbits (bv.of_N 42)) ∗ ⊤
       )%exp.
 
     (* Time Example t_vc__femtohandler : 𝕊 [] := *)
@@ -302,10 +299,6 @@ Import BlockVerificationDerived2.
       (* let vc4 := Postprocessing.solve_uvars vc3 in *)
       (* let vc5 := Postprocessing.prune vc4 in *)
       (* vc5. *)
-    (* Import SymProp.notations. *)
-    (* Set Printing Depth 200. *)
-    (* Compute vc__femtohandler. *)
-    (* Print vc__femtohandler. *)
 
     Lemma sat__femtohandler : safeE vc__femtohandler.
     Proof.
@@ -369,7 +362,7 @@ Import BlockVerificationDerived2.
   (* Import Sound. *)
   Import BlockVerificationDerived2Sem.
 
-  Definition advAddrs : list (bv xlenbits) := bv.seqBv (bv.of_N 88) (lenAddr - 88).
+  Definition advAddrs : list (bv xlenbits) := bv.seqBv (bv.of_N 80) (lenAddr - 80).
 
   (* Lemma liveAddr_split : liveAddrs = seqZ minAddr 88 ++ advAddrs. *)
   (* Proof. *)
@@ -425,14 +418,14 @@ Import BlockVerificationDerived2.
 
   (* Definition ptsto_readonly `{sailGS Σ} addr v : iProp Σ := *)
   (*       inv.inv femto_inv_ns (interp_ptsto addr v). *)
-  Definition femto_inv_fortytwo `{sailGS Σ} : iProp Σ := @interp_ptstomem_readonly _ _ _ xlenbytes (bv.of_N 84) (bv.of_N 42).
+  Definition femto_inv_fortytwo `{sailGS Σ} : iProp Σ := @interp_ptstomem_readonly _ _ _ xlenbytes (bv.of_N 76) (bv.of_N 42).
 
   Local Notation "a '↦' t" := (reg_pointsTo a t) (at level 79).
   (* Local Notation "a '↦ₘ' t" := (interp_ptsto a t) (at level 79). *)
 
   Definition femto_handler_pre `{sailGS Σ} : iProp Σ :=
       (mstatus ↦ {| MPP := User |}) ∗
-      (mtvec ↦ (bv.of_N 72)) ∗
+      (mtvec ↦ (bv.of_N 64)) ∗
       (∃ v, mcause ↦ v) ∗
       (∃ epc, mepc ↦ epc) ∗
       cur_privilege ↦ Machine ∗
@@ -440,13 +433,13 @@ Import BlockVerificationDerived2.
       interp_pmp_entries femto_pmpentries ∗
       interp_pmp_addr_access liveAddrs femto_pmpentries User ∗
       femto_inv_fortytwo ∗
-      pc ↦ (bv.of_N 72) ∗
+      pc ↦ (bv.of_N 64) ∗
       (∃ v, nextpc ↦ v) ∗
-      ptsto_instrs (bv.of_N 72) femtokernel_handler.
+      ptsto_instrs (bv.of_N 64) femtokernel_handler.
 
     Example femto_handler_post `{sailGS Σ} : iProp Σ :=
       (mstatus ↦ {| MPP := User |}) ∗
-        (mtvec ↦ (bv.of_N 72)) ∗
+        (mtvec ↦ (bv.of_N 64)) ∗
         (∃ v, mcause ↦ v) ∗
         cur_privilege ↦ User ∗
         interp_gprs ∗
@@ -456,7 +449,7 @@ Import BlockVerificationDerived2.
         (∃ epc, mepc ↦ epc ∗
                 pc ↦ epc) ∗
         (∃ v, nextpc ↦ v) ∗
-        ptsto_instrs (bv.of_N 72) femtokernel_handler.
+        ptsto_instrs (bv.of_N 64) femtokernel_handler.
 
   Definition femto_handler_contract `{sailGS Σ} : iProp Σ :=
     femto_handler_pre -∗
@@ -470,7 +463,7 @@ Import BlockVerificationDerived2.
   Lemma femto_handler_verified : forall `{sailGS Σ}, ⊢ femto_handler_contract.
   Proof.
     iIntros (Σ sG) "Hpre Hk".
-    iApply (sound_VC__addr $! (bv.of_N 72) with "[Hpre] [Hk]").
+    iApply (sound_VC__addr $! (bv.of_N 64) with "[Hpre] [Hk]").
     - exact sat__femtohandler.
     Unshelve.
     exact [env].
@@ -503,18 +496,18 @@ Import BlockVerificationDerived2.
 
   Lemma femtokernel_hander_safe `{sailGS Σ} :
     ⊢ mstatus ↦ {| MPP := User |} ∗
-       (mtvec ↦ (bv.of_N 72)) ∗
+       (mtvec ↦ (bv.of_N 64)) ∗
         (∃ v, mcause ↦ v) ∗
         (∃ mepcv, mepc ↦ mepcv) ∗
         cur_privilege ↦ Machine ∗
         interp_gprs ∗
         interp_pmp_entries femto_pmpentries ∗
         femto_inv_fortytwo ∗
-        (pc ↦ (bv.of_N 72)) ∗
+        (pc ↦ (bv.of_N 64)) ∗
         interp_pmp_addr_access liveAddrs femto_pmpentries User ∗
         (∃ v, nextpc ↦ v) ∗
         (* ptsto_instrs 0 femtokernel_init ∗  (domi: init code not actually needed anymore, can be dropped) *)
-        ptsto_instrs (bv.of_N 72) femtokernel_handler
+        ptsto_instrs (bv.of_N 64) femtokernel_handler
         -∗
         WP_loop.
   Proof.
@@ -549,20 +542,20 @@ Import BlockVerificationDerived2.
 
   Lemma femtokernel_manualStep2 `{sailGS Σ} :
     ⊢ (∃ mpp, mstatus ↦ {| MPP := mpp |}) ∗
-       (mtvec ↦ (bv.of_N 72)) ∗
+       (mtvec ↦ (bv.of_N 64)) ∗
         (∃ v, mcause ↦ v) ∗
         (∃ v, mepc ↦ v) ∗
         cur_privilege ↦ User ∗
         interp_gprs ∗
         interp_pmp_entries femto_pmpentries ∗
-         (@interp_ptstomem_readonly _ _ _ xlenbytes (bv.of_N 84) (bv.of_N 42)) ∗
-        (pc ↦ (bv.of_N 88)) ∗
+         (@interp_ptstomem_readonly _ _ _ xlenbytes (bv.of_N 76) (bv.of_N 42)) ∗
+        (pc ↦ (bv.of_N 80)) ∗
         (∃ v, nextpc ↦ v) ∗
         (* ptsto_instrs 0 femtokernel_init ∗  (domi: init code not actually needed anymore, can be dropped) *)
-        ptsto_instrs (bv.of_N 72) femtokernel_handler ∗
+        ptsto_instrs (bv.of_N 64) femtokernel_handler ∗
         ptstoSthL advAddrs
         ={⊤}=∗
-        ∃ mpp, LoopVerification.loop_pre User (bv.of_N 72) (bv.of_N 88) mpp femto_pmpentries.
+        ∃ mpp, LoopVerification.loop_pre User (bv.of_N 64) (bv.of_N 80) mpp femto_pmpentries.
   Proof.
     iIntros "([%mpp Hmst] & Hmtvec & [%mcause Hmcause] & [%mepc Hmepc] & Hcurpriv & Hgprs & Hpmpcfg & Hfortytwo & Hpc & Hnpc & Hhandler & Hmemadv)".
     iExists mpp.
@@ -610,24 +603,24 @@ Import BlockVerificationDerived2.
       pmp1cfg ↦ default_pmpcfg_ent ∗
       (pmpaddr0 ↦ bv.zero) ∗
       (pmpaddr1 ↦ bv.zero) ∗
-      interp_ptstomem_readonly (width := xlenbytes) (bv.of_N 84) (bv.of_N 42)) ∗
+      interp_ptstomem_readonly (width := xlenbytes) (bv.of_N 76) (bv.of_N 42)) ∗
       pc ↦ bv.zero ∗
       (∃ v, nextpc ↦ v) ∗
       ptsto_instrs bv.zero femtokernel_init.
 
     Example femto_init_post `{sailGS Σ} : iProp Σ :=
       ((∃ v, mstatus ↦ v) ∗
-        (mtvec ↦ (bv.of_N 72)) ∗
+        (mtvec ↦ (bv.of_N 64)) ∗
         (∃ v, mcause ↦ v) ∗
         (∃ v, mepc ↦ v) ∗
         cur_privilege ↦ User ∗
         interp_gprs ∗
         pmp0cfg ↦ femto_pmpcfg_ent0 ∗
         pmp1cfg ↦ femto_pmpcfg_ent1 ∗
-        (pmpaddr0 ↦ (bv.of_N 88)) ∗
+        (pmpaddr0 ↦ (bv.of_N 80)) ∗
         (pmpaddr1 ↦ (bv.of_N femto_address_max)) ∗
-        interp_ptstomem_readonly (width := xlenbytes) (bv.of_N 84) (bv.of_N 42)) ∗
-        pc ↦ (bv.of_N 88) ∗
+        interp_ptstomem_readonly (width := xlenbytes) (bv.of_N 76) (bv.of_N 42)) ∗
+        pc ↦ (bv.of_N 80) ∗
         (∃ v, nextpc ↦ v) ∗
         ptsto_instrs bv.zero femtokernel_init.
 
@@ -670,11 +663,11 @@ Import BlockVerificationDerived2.
       reg_pointsTo pmp1cfg default_pmpcfg_ent ∗
       (reg_pointsTo pmpaddr1 bv.zero) ∗
       (pc ↦ bv.zero) ∗
-      interp_ptstomem_readonly (width := xlenbytes) (bv.of_N 84) (bv.of_N 42) ∗
+      interp_ptstomem_readonly (width := xlenbytes) (bv.of_N 76) (bv.of_N 42) ∗
       ptstoSthL advAddrs ∗
       (∃ v, nextpc ↦ v) ∗
       ptsto_instrs bv.zero femtokernel_init ∗
-      ptsto_instrs (bv.of_N 72) femtokernel_handler
+      ptsto_instrs (bv.of_N 64) femtokernel_handler
       -∗
       WP_loop.
   Proof.
@@ -711,7 +704,7 @@ Import BlockVerificationDerived2.
   Import iris.bi.big_op.
   Import iris.algebra.big_op.
 
-  Lemma liveAddrs_split : liveAddrs = bv.seqBv (bv.of_N 0) 72 ++ bv.seqBv (bv.of_N 72) 12 ++ bv.seqBv (bv.of_N 84) 4 ++ advAddrs.
+  Lemma liveAddrs_split : liveAddrs = bv.seqBv (bv.of_N 0) 64 ++ bv.seqBv (bv.of_N 64) 12 ++ bv.seqBv (bv.of_N 76) 4 ++ advAddrs.
   Proof.
     (* TODO: scalable proof *)
     by compute.
@@ -804,12 +797,12 @@ Import BlockVerificationDerived2.
 
   Lemma femtokernel_splitMemory `{sailGS Σ} {μ : Memory} :
     mem_has_instrs μ (bv.of_N 0) femtokernel_init ->
-    mem_has_instrs μ (bv.of_N 72) femtokernel_handler ->
-    mem_has_word μ (bv.of_N 84) (bv.of_N 42) ->
+    mem_has_instrs μ (bv.of_N 64) femtokernel_handler ->
+    mem_has_word μ (bv.of_N 76) (bv.of_N 42) ->
     @mem_res _ sailGS_memGS μ ⊢ |={⊤}=>
       ptsto_instrs (bv.of_N 0) femtokernel_init ∗
-      ptsto_instrs (bv.of_N 72) femtokernel_handler ∗
-      interp_ptstomem_readonly (width := xlenbytes) (bv.of_N 84) (bv.of_N 42) ∗
+      ptsto_instrs (bv.of_N 64) femtokernel_handler ∗
+      interp_ptstomem_readonly (width := xlenbytes) (bv.of_N 76) (bv.of_N 42) ∗
       ptstoSthL advAddrs.
   Proof.
     iIntros (Hinit Hhandler Hft) "Hmem".
@@ -822,9 +815,9 @@ Import BlockVerificationDerived2.
     iSplitL "Hhandler".
     now iApply (intro_ptsto_instrs (μ := μ)).
     iSplitL "Hfortytwo".
-    - iAssert (interp_ptstomem (bv.of_N 84) (bv.of_N 42)) with "[Hfortytwo]" as "Hfortytwo".
+    - iAssert (interp_ptstomem (bv.of_N 76) (bv.of_N 42)) with "[Hfortytwo]" as "Hfortytwo".
       { now iApply (intro_ptstomem_word2 Hft with "Hfortytwo"). }
-      iMod (inv.inv_alloc femto_inv_ns ⊤ (interp_ptstomem (bv.of_N 84) (bv.of_N 42)) with "Hfortytwo") as "Hinv".
+      iMod (inv.inv_alloc femto_inv_ns ⊤ (interp_ptstomem (bv.of_N 76) (bv.of_N 42)) with "Hfortytwo") as "Hinv".
       now iModIntro.
     - now iApply (intro_ptstoSthL μ).
   Qed.
@@ -842,8 +835,8 @@ Import BlockVerificationDerived2.
   Lemma femtokernel_endToEnd {γ γ' : RegStore} {μ μ' : Memory}
         {δ δ' : CStore [ctx]} {s' : Stm [ctx] ty.unit} :
     mem_has_instrs μ (bv.of_N 0) femtokernel_init ->
-    mem_has_instrs μ (bv.of_N 72) femtokernel_handler ->
-    mem_has_word μ (bv.of_N 84) (bv.of_N 42) ->
+    mem_has_instrs μ (bv.of_N 64) femtokernel_handler ->
+    mem_has_word μ (bv.of_N 76) (bv.of_N 42) ->
     read_register γ cur_privilege = Machine ->
     read_register γ pmp0cfg = default_pmpcfg_ent ->
     read_register γ pmpaddr0 = bv.zero ->
@@ -851,10 +844,10 @@ Import BlockVerificationDerived2.
     read_register γ pmpaddr1 = bv.zero ->
     read_register γ pc = (bv.of_N 0) ->
     ⟨ γ, μ, δ, fun_loop ⟩ --->* ⟨ γ', μ', δ', s' ⟩ ->
-    μ' (bv.of_N 84) = (bv.of_N 42).
+    μ' (bv.of_N 76) = (bv.of_N 42).
   Proof.
     intros μinit μhandler μft γcurpriv γpmp0cfg γpmpaddr0 γpmp1cfg γpmpaddr1 γpc steps.
-    refine (adequacy_gen (Q := fun _ _ _ _ => True%I) (μ' (bv.of_N 84) = (bv.of_N 42)) steps _).
+    refine (adequacy_gen (Q := fun _ _ _ _ => True%I) (μ' (bv.of_N 76) = (bv.of_N 42)) steps _).
     iIntros (Σ' H).
     unfold own_regstore.
     cbn.
